Recover adequacy

syntax.sig
@@ -14,3 +14,4 @@ tRefl : tm
 tSig : T -> tm -> (tm -> tm) -> tm
 tPack : T -> tm -> tm -> tm
 tLet : T -> T -> tm -> (tm -> tm -> tm) -> tm
+tD : tm
